theories/lang/lib/spawn.v
@@ -108,7 +108,7 @@ Proof.
     - iModIntro. iApply wp_if. iNext. iApply ("IH" with "Hj H†").
       auto. }
   iDestruct "Ho" as (v) "(Hd & HΨ & Hf)".
-  iMod ("Hclose" with "[Hj Hf]").
+  iMod ("Hclose" with "[Hj Hf]") as "_".
   { iNext. iLeft. iFrame. }
   iModIntro. iApply wp_if. iNext. wp_op. wp_read. wp_let.
   iAssert (c ↦∗ [ #true; v])%I with "[Hc Hd]" as "Hc".
